src/model/thread_info.v
@@ -6,11 +6,17 @@ From compcert Require Import common.Values.
 
 From VST Require Import floyd.sublist.
 From VST Require Import msl.Coqlib2.
+From VST Require Import veric.base.
 From VST Require Import veric.val_lemmas.
+
+From CertiGraph Require Export graph.graph_gen.
 
 From CertiGC Require Import model.constants.
 From CertiGC Require Import model.graph.
 From CertiGC Require Import model.heap.
+From CertiGC Require Import model.util.
+
+Import ListNotations.
 
 
 Record thread_info: Type := {
@@ -69,6 +75,51 @@ Proof.
 Qed.
 
 
+Definition nth_gen_size (n: nat) := (NURSERY_SIZE * two_p (Z.of_nat n))%Z.
+
+Definition nth_gen_size_spec (tinfo: thread_info) (n: nat): Prop :=
+  if Val.eq (nth_space tinfo n).(space_base) nullval
+  then True
+  else gen_size tinfo n = nth_gen_size n.
+
+Definition ti_size_spec (tinfo: thread_info): Prop :=
+  Forall (nth_gen_size_spec tinfo) (nat_inc_list (Z.to_nat MAX_SPACES)).
+
+Definition safe_to_copy_gen g from to: Prop :=
+  nth_gen_size from <= nth_gen_size to - graph_gen_size g to.
+
+Lemma ngs_range: forall i,
+    0 <= i < MAX_SPACES -> 0 <= nth_gen_size (Z.to_nat i) < MAX_SPACE_SIZE.
+Proof.
+  intros. unfold nth_gen_size. rewrite MAX_SPACES_eq in H.
+  rewrite Z2Nat.id, NURSERY_SIZE_eq, Zbits.Zshiftl_mul_two_p,
+  Z.mul_1_l, <- two_p_is_exp by lia. split.
+  - cut (two_p (16 + i) > 0). 1: intros; lia. apply two_p_gt_ZERO. lia.
+  - transitivity (two_p 28). 1: apply two_p_monotone_strict; lia.
+    vm_compute. reflexivity.
+Qed.
+
+Lemma ngs_int_singed_range: forall i,
+    0 <= i < MAX_SPACES ->
+    (if Archi.ptr64 then Int64.min_signed else Int.min_signed) <=
+    nth_gen_size (Z.to_nat i) <=
+    (if Archi.ptr64 then Int64.max_signed else Int.max_signed).
+Proof.
+  intros. apply ngs_range in H. destruct H. split.
+  - transitivity 0. 2: assumption. vm_compute. intro HS; inversion HS.
+  - apply Z.lt_le_incl. transitivity MAX_SPACE_SIZE. 1: assumption.
+    unfold MAX_SPACE_SIZE. vm_compute. reflexivity.
+Qed.
+
+Lemma ngs_S: forall i,
+    0 <= i -> 2 * nth_gen_size (Z.to_nat i) = nth_gen_size (Z.to_nat (i + 1)).
+Proof.
+  intros. unfold nth_gen_size. rewrite !Z2Nat.id by lia.
+  rewrite Z.mul_comm, <- Z.mul_assoc, (Z.mul_comm (two_p i)), <- two_p_S by assumption.
+  reflexivity.
+Qed.
+
+
 Record fun_info : Type := {
     fun_word_size: Z;
     live_roots_indices: list Z;
@@ -76,3 +127,27 @@ Record fun_info : Type := {
     lri_range: (Zlength (live_roots_indices) <= MAX_UINT - 2)%Z;
     word_size_range: (0 <= fun_word_size <= MAX_UINT)%Z;
 }.
+
+
+Definition np_roots_rel from f_info (roots roots': roots_t) (l: list Z) : Prop :=
+  let lri := live_roots_indices f_info in
+  let maped_lri := (map ((fun x y => Znth y x) lri) l) in
+  forall v j, Znth j roots' = inr v ->
+              (In (Znth j lri) maped_lri -> addr_gen v <> from) /\
+              (~ In (Znth j lri) maped_lri -> Znth j roots = inr v).
+
+Lemma np_roots_rel_cons: forall roots1 roots2 roots3 from f_info i l,
+    np_roots_rel from f_info roots1 roots2 [i] ->
+    np_roots_rel from f_info roots2 roots3 l ->
+    np_roots_rel from f_info roots1 roots3 (i :: l).
+Proof.
+  intros. unfold np_roots_rel in *. intros. simpl. specialize (H0 _ _ H1).
+  destruct H0. split; intros.
+  - destruct (in_dec Z.eq_dec (Znth j (live_roots_indices f_info))
+                     (map ((fun x y => Znth y x) (live_roots_indices f_info)) l)).
+    1: apply H0; assumption. destruct H3. 2: contradiction.
+    specialize (H2 n). specialize (H _ _ H2). destruct H. apply H. simpl.
+    left; assumption.
+  - apply Decidable.not_or in H3. destruct H3.
+    specialize (H2 H4). specialize (H _ _ H2). destruct H. apply H5. simpl. tauto.
+Qed.
