src/model/forward.v
@@ -12,7 +12,7 @@ From VST Require Import veric.base.
 From VST Require Import veric.shares.
 From VST Require Import veric.val_lemmas.
 
-From CertiGraph Require Export graph.graph_gen.
+From CertiGraph Require Import graph.graph_gen.
 From CertiGraph Require Import graph.graph_model.
 From CertiGraph Require Import lib.EquivDec_ext.
 From CertiGraph Require Import lib.List_ext.
@@ -27,6 +27,7 @@ From CertiGC Require Import model.thread_info.
 From CertiGC Require Import model.update.
 From CertiGC Require Import model.util.
 
+Import ListNotations.
 Local Coercion pg_lg: LabeledGraph >-> PreGraph.
 
 
@@ -624,4 +625,389 @@ Proof.
   intros. unfold upd_roots. destruct p; [|assumption]. destruct (Znth z roots).
   1: destruct s; assumption. if_tac. 2: assumption.
   destruct (block_mark (vlabel g a)); apply upd_bunch_rf_compatible; assumption.
+Qed.
+
+
+Lemma upd_roots_not_pointing: forall from to i g roots f_info roots',
+    copy_compatible g -> roots_graph_compatible roots g -> from <> to ->
+    0 <= i < Zlength roots -> roots_fi_compatible roots f_info ->
+    roots' = upd_roots from to (inl i) g roots f_info ->
+    np_roots_rel from f_info roots roots' [i].
+Proof.
+  intros. unfold np_roots_rel. intros. simpl.
+  assert (Zlength roots' = Zlength roots) by
+      (rewrite H4; apply upd_roots_Zlength, (proj1 H3)).
+  assert (0 <= j < Zlength roots). {
+    rewrite <- H6. destruct (Z_lt_le_dec j (Zlength roots')).
+    2: rewrite Znth_outofbounds in H5 by lia; inversion H5. split; auto.
+    destruct (Z_lt_le_dec j 0); auto. rewrite Znth_outofbounds in H5 by lia.
+    inversion H5. } simpl in H4. destruct H3. destruct (Znth i roots) eqn:? .
+  - assert (roots' = roots) by (destruct s; assumption). clear H4. subst roots'.
+    split; intros; auto. destruct H4; auto.
+    destruct H3. apply H8 in H4; try assumption. rewrite Heqr, H5 in H4. inversion H4.
+  - if_tac in H4.
+    + destruct (block_mark (vlabel g a)) eqn: ?; subst; split; intros.
+      * destruct H4; auto. symmetry in H4. rewrite upd_bunch_same in H5 by assumption.
+        inversion H5. red in H0. rewrite Forall_forall in H0.
+        assert (graph_has_v g a). {
+          apply H0. rewrite <- filter_sum_right_In_iff, <- Heqr.
+          apply Znth_In; assumption. } destruct (H _ H9 Heqb) as [_ ?]. auto.
+      * assert (Znth j (live_roots_indices f_info) <>
+                Znth i (live_roots_indices f_info)) by intuition. clear H4.
+        rewrite upd_bunch_diff in H5; assumption.
+      * destruct H4; auto. symmetry in H4. rewrite upd_bunch_same in H5 by assumption.
+        inversion H5. unfold new_copied_v. simpl. auto.
+      * assert (Znth j (live_roots_indices f_info) <>
+                Znth i (live_roots_indices f_info)) by intuition. clear H4.
+        rewrite upd_bunch_diff in H5; assumption.
+    + split; intros; subst roots'; auto. destruct H10; auto.
+      apply H8 in H4; try assumption. rewrite Heqr, H5 in H4. inversion H4.
+      subst a. assumption.
+Qed.
+
+
+Lemma fr_copy_compatible: forall depth from to p g g',
+    from <> to -> graph_has_gen g to -> forward_relation from to depth p g g' ->
+    copy_compatible g -> copy_compatible g'.
+Proof.
+  intros. remember (fun (g: HeapGraph) (v: Addr) (x: nat) => True) as Q.
+  remember (fun g1 g2 (v: Addr) => copy_compatible g1 -> copy_compatible g2) as P.
+  remember (fun (x y: nat) => x <> y) as R.
+  pose proof (fr_general_prop depth from to p g g' _ Q P R). subst Q P R.
+  apply H3; clear H3; intros; try assumption; try reflexivity.
+  - apply H4, H3. assumption.
+  - subst from0. apply lcv_copy_compatible; auto.
+  - exact {| addr_gen := O; addr_block := O |}.
+Qed.
+
+Lemma fr_right_roots_graph_compatible: forall depth from to e g g' roots,
+    graph_has_gen g to -> forward_p_compatible (inr e) roots g from ->
+    forward_relation from to depth (forward_p2forward_t (inr e) [] g) g g' ->
+    roots_graph_compatible roots g -> roots_graph_compatible roots g'.
+Proof.
+  intros. simpl in H1, H0. destruct e. destruct H0 as [_ [_ [? _]]]. rewrite H0 in H1.
+  simpl in H1. remember (fun (g: HeapGraph) (v: nat) (x: nat) => True) as Q.
+  remember (fun g1 g2 (x: nat) => roots_graph_compatible roots g1->
+                                  roots_graph_compatible roots g2) as P.
+  remember (fun (x1 x2: nat) => True) as R.
+  pose proof (fr_general_prop
+                depth from to (field2forward (Znth z (make_fields g a))) g g' _ Q P R).
+  subst Q P R. apply H3; clear H3; intros; try assumption; try reflexivity.
+  - apply H4, H3. assumption.
+  - apply lcv_rgc_unchanged; assumption.
+Qed.
+
+Lemma fl_edge_roots_graph_compatible: forall depth from to l g g' v roots,
+    addr_gen v <> from ->
+    graph_has_gen g to -> graph_has_v g v -> block_mark (vlabel g v) = false ->
+    forward_loop from to depth (map (fun x : nat => inr (v, Z.of_nat x)) l) g g' ->
+    (forall i, In i l -> i < length (block_fields (vlabel g v)))%nat ->
+    roots_graph_compatible roots g -> roots_graph_compatible roots g'.
+Proof.
+  do 4 intro. induction l; intros; simpl in H3; inversion H3; subst. 1: assumption.
+  cut (roots_graph_compatible roots g2).
+  - intros. apply (IHl g2 _ v); try assumption.
+    + rewrite <- fr_graph_has_gen; eauto.
+    + eapply fr_graph_has_v; eauto.
+    + rewrite <- H2. symmetry. eapply fr_block_mark; eauto.
+    + assert (block_fields (vlabel g v) = block_fields (vlabel g2 v)) by
+          (eapply fr_block_fields; eauto). rewrite <- H7.
+      intros; apply H4; right; assumption.
+  - specialize (H4 _ (in_eq a l)). eapply fr_right_roots_graph_compatible; eauto.
+    simpl. intuition. rewrite Zlength_correct. apply inj_lt; assumption.
+Qed.
+
+Lemma fr_roots_outlier_compatible: forall from to p g roots f_info outlier,
+    roots_outlier_compatible roots outlier ->
+    roots_outlier_compatible (upd_roots from to p g roots f_info) outlier.
+Proof.
+  intros. destruct p; simpl in *. 2: assumption. destruct (Znth z roots) eqn: ?.
+  + destruct s; assumption.
+  + if_tac. 2: assumption.
+    destruct (block_mark (vlabel g a)); apply upd_roots_outlier_compatible; assumption.
+Qed.
+
+Lemma fr_roots_graph_compatible (depth from to: nat) (p : forward_p_type) (g g' : HeapGraph) (roots : roots_t) (f_info : fun_info)
+    (Hto: graph_has_gen g to)
+    (Hp: forward_p_compatible p roots g from)
+    (Hg: copy_compatible g)
+    (Hfwd: forward_relation from to depth (forward_p2forward_t p roots g) g g')
+    (Hfrom_to: from <> to)
+    (Hroots: roots_graph_compatible roots g):
+    roots_graph_compatible (upd_roots from to p g roots f_info) g'.
+Proof.
+  destruct p.
+  - simpl in *. destruct (Znth z roots) eqn: ?; simpl in *.
+    + destruct s; inversion Hfwd; subst; assumption.
+    + assert (graph_has_v g a). {
+        red in Hroots. rewrite Forall_forall in Hroots. apply Hroots.
+        rewrite <- filter_sum_right_In_iff. rewrite <- Heqr. apply Znth_In.
+        assumption. }
+      inversion Hfwd ; destruct (Nat.eq_dec (addr_gen v) from) eqn:HE_v_from ; subst ; rewrite HE_v_from ; try easy.
+      * rename H3 into Eblock_mark ; rewrite Eblock_mark.
+        apply upd_bunch_graph_compatible ; try assumption.
+        now apply Hg.
+      * rename H3 into Eblock_mark ; rewrite Eblock_mark.
+        now apply lcv_roots_graph_compatible.
+      * rename H2 into Eblock_mark ; rewrite Eblock_mark.
+        assert (graph_has_v new_g (new_copied_v g to)) by
+          (subst new_g; apply lcv_graph_has_v_new; assumption).
+        remember (nat_inc_list (length (block_fields (vlabel new_g (new_copied_v g to))))) as new_fields.
+        assert (graph_has_v new_g (new_copied_v g to)) by (subst new_g; apply lcv_graph_has_v_new; assumption).
+        remember (upd_bunch z f_info roots (inr (new_copied_v g to))) as roots'.
+        assert (roots_graph_compatible roots' new_g) by (subst; subst new_g; apply lcv_roots_graph_compatible; assumption).
+        assert (block_mark (vlabel new_g (new_copied_v g to)) = false). {
+          subst new_g. unfold lgraph_copy_v. rewrite <- lmc_block_mark.
+          - now rewrite lacv_vlabel_new.
+          - unfold new_copied_v. destruct a. destruct Heqroots'. simpl in *.
+            red in H1. intro HS. inversion HS. lia. }
+        eapply (fl_edge_roots_graph_compatible depth0 (addr_gen a) to new_fields new_g _ (new_copied_v g to)) ; eauto.
+        -- subst new_g. now rewrite <- lcv_graph_has_gen.
+        -- now subst new_fields.
+        -- intros idx Hidx. subst new_fields. now rewrite nat_inc_list_In_iff in Hidx.
+  - simpl. eapply fr_right_roots_graph_compatible; eauto.
+Qed.
+
+Lemma fr_roots_compatible: forall depth from to p g g' roots f_info outlier,
+    graph_has_gen g to -> forward_p_compatible p roots g from -> copy_compatible g ->
+    forward_relation from to depth (forward_p2forward_t p roots g) g g' ->
+    roots_compatible g outlier roots -> from <> to ->
+    roots_compatible g' outlier (upd_roots from to p g roots f_info).
+Proof.
+  intros. destruct H3. split.
+  - apply fr_roots_outlier_compatible; assumption.
+  - eapply fr_roots_graph_compatible; eauto.
+Qed.
+
+Lemma frl_not_pointing: forall from to f_info l roots1 g1 roots2 g2,
+    copy_compatible g1 -> roots_graph_compatible roots1 g1 -> from <> to ->
+    (forall i, In i l -> i < length roots1)%nat -> roots_fi_compatible roots1 f_info ->
+    forward_roots_loop from to f_info l roots1 g1 roots2 g2 -> graph_has_gen g1 to ->
+    np_roots_rel from f_info roots1 roots2 (map Z.of_nat l).
+Proof.
+  do 4 intro. induction l; intros; inversion H4; subst.
+  1: red; simpl; intros; intuition.
+  remember (upd_roots from to (inl (Z.of_nat a)) g1 roots1 f_info) as roots3.
+  simpl. apply np_roots_rel_cons with roots3.
+  - apply (upd_roots_not_pointing from to _ g1); try assumption.
+    split. 1: lia. rewrite Zlength_correct. apply inj_lt. apply H2. left; auto.
+  - assert (Zlength roots3 = Zlength roots1) by
+        (subst roots3; apply upd_roots_Zlength; apply (proj1 H3)).
+    apply (IHl _ g3 _ g2); auto.
+    + apply fr_copy_compatible in H8; assumption.
+    + subst roots3. eapply fr_roots_graph_compatible; eauto. simpl. split. 1: lia.
+      specialize (H2 _ (in_eq a l)). rewrite Zlength_correct. apply inj_lt; assumption.
+    + intros. subst roots3. rewrite <- ZtoNat_Zlength, H6, ZtoNat_Zlength.
+      apply H2; right; assumption.
+    + subst roots3; apply upd_roots_rf_compatible; assumption.
+    + rewrite <- (fr_graph_has_gen _ _ _ _ _ _ H5 H8); assumption.
+Qed.
+
+
+Lemma frr_not_pointing: forall from to f_info roots1 g1 roots2 g2,
+    copy_compatible g1 -> roots_graph_compatible roots1 g1 -> from <> to ->
+    graph_has_gen g1 to -> roots_fi_compatible roots1 f_info ->
+    forward_roots_relation from to f_info roots1 g1 roots2 g2 ->
+    roots_have_no_gen roots2 from.
+Proof.
+  intros. unfold forward_roots_relation in H0. eapply frl_not_pointing in H0; eauto.
+  red; intros. 2: intros; rewrite nat_inc_list_In_iff in H5; assumption. red in H0.
+  apply In_Znth in H5. destruct H5 as [i [? ?]]. specialize (H0 _ _ H6). destruct H0.
+  apply H0. destruct H3 as [? _].
+  replace (length roots1) with (length (live_roots_indices f_info)) by
+      (rewrite <- !ZtoNat_Zlength, H3; reflexivity).
+  remember (live_roots_indices f_info). rewrite map_map.
+  assert (map (fun x : nat => Znth (Z.of_nat x) l) (nat_inc_list (length l)) = l). {
+    clear. rewrite Znth_list_eq. split.
+    - rewrite Zlength_map, !Zlength_correct, nat_inc_list_length. reflexivity.
+    - intros. rewrite Zlength_map in H. rewrite Znth_map by assumption. f_equal.
+      rewrite <- nth_Znth by assumption. rewrite nat_inc_list_nth.
+      1: apply Z2Nat.id; lia. rewrite Zlength_correct, nat_inc_list_length in H.
+      rep_lia. } rewrite H8. clear H8. apply Znth_In. apply frl_roots_Zlength in H4.
+  2: subst; assumption. rewrite <- H3, <- H4. assumption.
+Qed.
+
+
+Lemma frr_graph_has_gen: forall from to f_info roots1 g1 roots2 g2,
+    graph_has_gen g1 to ->
+    forward_roots_relation from to f_info roots1 g1 roots2 g2 ->
+    forall gen, graph_has_gen g1 gen <-> graph_has_gen g2 gen.
+Proof.
+  intros. induction H0. 1: reflexivity. rewrite <- IHforward_roots_loop.
+  - eapply fr_graph_has_gen; eauto.
+  - rewrite <- fr_graph_has_gen; eauto.
+Qed.
+
+
+Lemma fr_O_dst_unchanged_root: forall from to r g g',
+    forward_relation from to O (root2forward r) g g' ->
+    forall e, graph_has_v g (field_addr e) -> dst g e = dst g' e.
+Proof.
+  intros. destruct r; [destruct s|]; simpl in H; inversion H; subst; try reflexivity.
+  simpl. rewrite pcv_dst_old. 1: reflexivity. destruct e as [[gen vidx] eidx].
+  unfold graph_has_v in H0. unfold new_copied_v. simpl in *. destruct H0. intro.
+  inversion H2. subst. red in H1. lia.
+Qed.
+
+Lemma frr_dst_unchanged: forall from to f_info roots1 g1 roots2 g2,
+    graph_has_gen g1 to -> forward_roots_relation from to f_info roots1 g1 roots2 g2 ->
+    forall e, graph_has_v g1 (field_addr e) -> dst g1 e = dst g2 e.
+Proof.
+  intros. induction H0. 1: reflexivity. rewrite <- IHforward_roots_loop.
+  - eapply fr_O_dst_unchanged_root; eauto.
+  - rewrite <- fr_graph_has_gen; eauto.
+  - eapply fr_graph_has_v; eauto.
+Qed.
+
+Lemma fr_O_graph_has_v_inv: forall from to p g g',
+    graph_has_gen g to -> forward_relation from to O p g g' ->
+    forall v, graph_has_v g' v -> graph_has_v g v \/ v = new_copied_v g to.
+Proof.
+  intros. inversion H0; subst; try (left; assumption);
+            [|subst new_g; rewrite <- lgd_graph_has_v in H1];
+            apply lcv_graph_has_v_inv in H1; assumption.
+Qed.
+
+
+Lemma fr_O_gen_v_num_to: forall from to p g g',
+    graph_has_gen g to -> forward_relation from to O p g g' ->
+    (gen_v_num g to <= gen_v_num g' to)%nat.
+Proof.
+  intros. inversion H0; subst; try lia; [|subst new_g..].
+  - apply lcv_gen_v_num_to; auto.
+  - rewrite lgd_gen_v_num_to. lia.
+  - rewrite lgd_gen_v_num_to. apply lcv_gen_v_num_to. assumption.
+Qed.
+
+Lemma frr_gen_v_num_to: forall from to f_info roots1 g1 roots2 g2,
+    graph_has_gen g1 to -> forward_roots_relation from to f_info roots1 g1 roots2 g2 ->
+    (gen_v_num g1 to <= gen_v_num g2 to)%nat.
+Proof.
+  intros. induction H0. 1: lia. transitivity (gen_v_num g2 to).
+  - eapply fr_O_gen_v_num_to; eauto.
+  - apply IHforward_roots_loop; rewrite <- fr_graph_has_gen; eauto.
+Qed.
+
+Lemma frr_graph_has_v_inv: forall from to f_info roots1 g1 roots2 g2,
+    graph_has_gen g1 to -> forward_roots_relation from to f_info roots1 g1 roots2 g2 ->
+    forall v, graph_has_v g2 v -> graph_has_v g1 v \/
+                                  (addr_gen v = to /\
+                                   gen_v_num g1 to <= addr_block v < gen_v_num g2 to)%nat.
+Proof.
+  intros. induction H0. 1: left; assumption.
+  assert (graph_has_gen g2 to) by (rewrite <- fr_graph_has_gen; eauto).
+  specialize (IHforward_roots_loop H3 H1). destruct IHforward_roots_loop.
+  - eapply (fr_O_graph_has_v_inv from to _ g1 g2) in H0; eauto. destruct H0.
+    1: left; assumption. right. unfold new_copied_v in H0. subst v.
+    clear H2. destruct H1. red in H1. simpl in *. unfold gen_v_num. lia.
+  - right. destruct H4. split. 1: assumption. destruct H5. split. 2: assumption.
+    apply fr_O_gen_v_num_to in H0; [lia | assumption].
+Qed.
+
+Lemma frr_block_fields: forall from to f_info roots1 g1 roots2 g2,
+    graph_has_gen g1 to -> forward_roots_relation from to f_info roots1 g1 roots2 g2 ->
+    forall v, graph_has_v g1 v -> block_fields (vlabel g1 v) = block_fields (vlabel g2 v).
+Proof.
+  intros. induction H0. 1: reflexivity. rewrite <- IHforward_roots_loop.
+  - eapply fr_block_fields; eauto.
+  - rewrite <- fr_graph_has_gen; eauto.
+  - eapply fr_graph_has_v; eauto.
+Qed.
+
+Lemma frr_gen2gen_no_edge: forall from to f_info roots1 g1 roots2 g2,
+    graph_has_gen g1 to -> forward_roots_relation from to f_info roots1 g1 roots2 g2 ->
+    forall gen1 gen2, gen1 <> to -> gen2gen_no_edge g1 gen1 gen2 ->
+                      gen2gen_no_edge g2 gen1 gen2.
+Proof.
+  intros. unfold gen2gen_no_edge in *. intros.
+  cut (graph_has_e g1 {| field_addr := {| addr_gen := gen1; addr_block := vidx |} ; field_index := eidx |}).
+  - intros. erewrite <- frr_dst_unchanged; eauto. destruct H4. assumption.
+  - destruct H3. eapply frr_graph_has_v_inv in H3; eauto. destruct H3 as [? | [? ?]].
+    2: simpl in H3; contradiction. split. 1: simpl; assumption. simpl in *.
+    cut (get_edges g1 {| addr_gen := gen1 ; addr_block := vidx |} = get_edges g2 {| addr_gen := gen1 ; addr_block := vidx |}).
+    + intros; rewrite H5; assumption.
+    + unfold get_edges. unfold make_fields. erewrite frr_block_fields; eauto.
+Qed.
+
+Lemma fr_O_dst_unchanged_field: forall from to v n g g',
+    forward_p_compatible (inr (v, Z.of_nat n)) [] g from ->
+    forward_relation from to O (forward_p2forward_t (inr (v, Z.of_nat n)) [] g) g g' ->
+    forall e, graph_has_v g (field_addr e) -> e <> {| field_addr := v; field_index := n |} -> dst g e = dst g' e.
+Proof.
+  intros. simpl in *. destruct H as [? [? [? ?]]]. rewrite H4 in H0. simpl in H0.
+  remember (Znth (Z.of_nat n) (make_fields g v)).
+  assert (forall e0, inr e0 = Znth (Z.of_nat n) (make_fields g v) -> e0 <> e). {
+    intros. symmetry in H6. apply make_fields_Znth_edge in H6. 2: assumption.
+    rewrite Nat2Z.id in H6. rewrite <- H6 in H2. auto. }
+  destruct f; [destruct s |]; simpl in H0; inversion H0; subst; try reflexivity.
+  - subst new_g. rewrite lgd_dst_old. 1: reflexivity. apply H6; assumption.
+  - subst new_g. rewrite lgd_dst_old. 2: apply H6; assumption. simpl.
+    rewrite pcv_dst_old. 1: reflexivity. intro. rewrite H7 in H1. destruct H1.
+    unfold new_copied_v in H8. simpl in H8. red in H8. lia.
+Qed.
+
+
+Lemma frr_graph_has_v: forall from to f_info roots1 g1 roots2 g2,
+    graph_has_gen g1 to -> forward_roots_relation from to f_info roots1 g1 roots2 g2 ->
+    forall v, graph_has_v g1 v -> graph_has_v g2 v.
+Proof.
+  intros. induction H0; subst. 1: assumption. cut (graph_has_v g2 v).
+  - intros. apply IHforward_roots_loop; auto. erewrite <- fr_graph_has_gen; eauto.
+  - eapply fr_graph_has_v; eauto.
+Qed.
+
+Lemma fr_O_dst_changed_field: forall from to v n g g',
+    copy_compatible g -> no_dangling_dst g -> from <> to -> graph_has_gen g to ->
+    forward_p_compatible (inr (v, Z.of_nat n)) [] g from ->
+    forward_relation from to O (forward_p2forward_t (inr (v, Z.of_nat n)) [] g) g g' ->
+    forall e, Znth (Z.of_nat n) (make_fields g' v) = inr e ->
+              addr_gen (dst g' e) <> from.
+Proof.
+  intros. simpl in *. destruct H3 as [? [? [? ?]]]. rewrite H7 in H4. simpl in H4.
+  assert (make_fields g v = make_fields g' v) by
+      (unfold make_fields; erewrite fr_block_fields; eauto). rewrite <- H9 in *.
+  clear H9. remember (Znth (Z.of_nat n) (make_fields g v)). destruct f; inversion H5.
+  subst. clear H5. symmetry in Heqf. pose proof Heqf.
+  apply make_fields_Znth_edge in Heqf. 2: assumption. simpl in H4. subst.
+  rewrite Nat2Z.id in *.
+  inversion H4; subst; try assumption; subst new_g; rewrite lgd_dst_new.
+  - apply H in H12. 1: destruct H12; auto. specialize (H0 _ H3). apply H0.
+    unfold get_edges. rewrite <- filter_sum_right_In_iff, <- H5. apply Znth_In.
+    rewrite make_fields_eq_length. assumption.
+  - unfold new_copied_v. simpl. auto.
+Qed.
+
+Lemma fr_O_no_dangling_dst: forall from to p g g' roots,
+    forward_p_compatible p roots g from -> graph_has_gen g to ->
+    roots_graph_compatible roots g -> copy_compatible g ->
+    forward_relation from to O (forward_p2forward_t p roots g) g g' ->
+    no_dangling_dst g -> no_dangling_dst g'.
+Proof.
+  intros. inversion H3; subst; try assumption.
+  - destruct p; simpl in H5.
+    + destruct (Znth z roots) eqn:? ; [destruct s|]; simpl in H5; inversion H5.
+      subst. clear H5. apply lcv_no_dangling_dst; auto. red in H1.
+      rewrite Forall_forall in H1. apply H1. rewrite <- filter_sum_right_In_iff.
+      rewrite <- Heqr. apply Znth_In. assumption.
+    + destruct p. simpl in H. destruct H as [? [? [? ?]]]. rewrite H8 in H5.
+      simpl in H5. destruct (Znth z (make_fields g a)); [destruct s|];
+                     simpl in H5; inversion H5.
+  - subst new_g. apply lgd_no_dangling_dst_copied_vert; auto.
+    destruct p; simpl in H5.
+    + destruct (Znth z roots); [destruct s|]; simpl in H5; inversion H5.
+    + destruct p. simpl in H. destruct H as [? [? [? ?]]]. rewrite H7 in H5.
+      simpl in H5. destruct (Znth z (make_fields g a)) eqn:? ; [destruct s|];
+                     simpl in H5; inversion H5. subst. clear H5.
+      specialize (H4 _ H). apply H4. unfold get_edges.
+      rewrite <- filter_sum_right_In_iff, <- Heqf. apply Znth_In.
+      rewrite make_fields_eq_length. assumption.
+  - subst new_g. apply lgd_no_dangling_dst. 1: apply lcv_graph_has_v_new; auto.
+    apply lcv_no_dangling_dst; auto. destruct p; simpl in H5.
+    + destruct (Znth z roots); [destruct s|]; simpl in H5; inversion H5.
+    + destruct p. simpl in H. destruct H as [? [? [? ?]]]. rewrite H8 in H5.
+      simpl in H5. destruct (Znth z (make_fields g a)) eqn:? ; [destruct s|];
+                     simpl in H5; inversion H5. subst. clear H5.
+      specialize (H4 _ H). apply H4. unfold get_edges.
+      rewrite <- filter_sum_right_In_iff, <- Heqf. apply Znth_In.
+      rewrite make_fields_eq_length. assumption.
 Qed.
