src/model/scan.v
@@ -1,0 +1,394 @@
+From Coq Require Import Logic.FinFun.
+From Coq Require Import Lists.List.
+From Coq Require Import micromega.Lia.
+From Coq Require Import ZArith.ZArith.
+
+From compcert Require Import common.Values.
+From compcert Require Import lib.Integers.
+
+From VST Require Import floyd.functional_base.
+From VST Require Import floyd.sublist.
+From VST Require Import msl.shares.
+From VST Require Import veric.base.
+From VST Require Import veric.shares.
+From VST Require Import veric.val_lemmas.
+
+From CertiGraph Require Import graph.graph_gen.
+From CertiGraph Require Import graph.graph_model.
+From CertiGraph Require Import lib.EquivDec_ext.
+From CertiGraph Require Import lib.List_ext.
+
+From CertiGC Require Import model.compatible.
+From CertiGC Require Import model.constants.
+From CertiGC Require Import model.copy.
+From CertiGC Require Import model.cut.
+From CertiGC Require Import model.forward.
+From CertiGC Require Import model.graph.
+From CertiGC Require Import model.heap.
+From CertiGC Require Import model.reset.
+From CertiGC Require Import model.thread_info.
+From CertiGC Require Import model.util.
+
+Local Coercion pg_lg: LabeledGraph >-> PreGraph.
+
+
+Inductive scan_vertex_for_loop (from to: nat) (v: Addr):
+  list nat -> HeapGraph -> HeapGraph -> Prop :=
+| svfl_nil: forall g, scan_vertex_for_loop from to v nil g g
+| svfl_cons: forall g1 g2 g3 i il,
+  forward_relation
+    from to O (forward_p2forward_t (inr (v, (Z.of_nat i))) nil g1) g1 g2 ->
+  scan_vertex_for_loop from to v il g2 g3 ->
+  scan_vertex_for_loop from to v (i :: il) g1 g3.
+
+
+Inductive scan_vertex_while_loop (from to: nat):
+  list nat -> HeapGraph -> HeapGraph -> Prop :=
+| svwl_nil: forall g, scan_vertex_while_loop from to nil g g
+| svwl_no_scan: forall g1 g2 i il,
+    gen_has_index g1 to i -> no_scan g1 {| addr_gen := to; addr_block := i |} ->
+    scan_vertex_while_loop from to il g1 g2 ->
+    scan_vertex_while_loop from to (i :: il) g1 g2
+| svwl_scan: forall g1 g2 g3 i il,
+    gen_has_index g1 to i -> ~ no_scan g1 {| addr_gen := to; addr_block := i|} ->
+    scan_vertex_for_loop
+      from to {| addr_gen := to; addr_block := i|}
+      (nat_inc_list (length (vlabel g1 {| addr_gen := to; addr_block := i|}).(block_fields))) g1 g2 ->
+    scan_vertex_while_loop from to il g2 g3 ->
+    scan_vertex_while_loop from to (i :: il) g1 g3.
+
+Definition do_scan_relation (from to to_index: nat) (g1 g2: HeapGraph) : Prop :=
+  exists n, scan_vertex_while_loop from to (nat_seq to_index n) g1 g2 /\
+            ~ gen_has_index g2 to (to_index + n).
+
+
+Lemma svfl_graph_has_gen: forall from to v l g g',
+    graph_has_gen g to -> scan_vertex_for_loop from to v l g g' ->
+    forall x, graph_has_gen g x <-> graph_has_gen g' x.
+Proof.
+  intros from to v l. revert from to v. induction l; intros; inversion H0; subst.
+  1: reflexivity. transitivity (graph_has_gen g2 x).
+  - eapply fr_graph_has_gen; eauto.
+  - apply (IHl from to v). 2: assumption. rewrite <- fr_graph_has_gen; eauto.
+Qed.
+
+Lemma svfl_gen_unmarked: forall from to v l g g',
+    graph_has_gen g to -> scan_vertex_for_loop from to v l g g' ->
+    forall gen, from <> gen -> gen_unmarked g gen -> gen_unmarked g' gen.
+Proof.
+  intros from to v l. revert from to v.
+  induction l; intros; inversion H0; subst; try assumption.
+  eapply (IHl from to _ g2); eauto.
+  - rewrite <- fr_graph_has_gen; eauto.
+  - eapply fr_gen_unmarked; eauto.
+Qed.
+
+Lemma svwl_gen_unmarked: forall from to l g g',
+    graph_has_gen g to -> scan_vertex_while_loop from to l g g' ->
+    forall gen, from <> gen -> gen_unmarked g gen -> gen_unmarked g' gen.
+Proof.
+  do 3 intro. induction l; intros; inversion H0; subst;
+                [| apply (IHl g) | apply (IHl g2)]; try assumption.
+  - rewrite <- svfl_graph_has_gen; eauto.
+  - eapply svfl_gen_unmarked; eauto.
+Qed.
+
+Lemma svfl_vertex_address: forall from to v l g g',
+    graph_has_gen g to -> scan_vertex_for_loop from to v l g g' ->
+    forall x, closure_has_v g x -> vertex_address g x = vertex_address g' x.
+Proof.
+  do 4 intro. revert from to v. induction l; intros; simpl; inversion H0; subst.
+  1: reflexivity. assert (graph_has_gen g2 to) by
+      (eapply fr_graph_has_gen in H4; [rewrite <- H4 |]; assumption).
+  assert (closure_has_v g2 x) by (eapply fr_closure_has_v in H4; eauto).
+  eapply (IHl from to _ g2) in H7; eauto. rewrite <- H7.
+  eapply fr_vertex_address; eauto.
+Qed.
+
+Lemma svfl_graph_has_v: forall from to v l g g',
+    graph_has_gen g to -> scan_vertex_for_loop from to v l g g' ->
+    forall x, graph_has_v g x -> graph_has_v g' x.
+Proof.
+  do 4 intro. revert from to v. induction l; intros; simpl; inversion H0; subst.
+  1: assumption. assert (graph_has_gen g2 to) by
+      (eapply fr_graph_has_gen in H4; [rewrite <- H4 |]; assumption).
+  assert (graph_has_v g2 x) by (eapply fr_graph_has_v in H4; eauto).
+  eapply (IHl from to _ g2) in H7; eauto.
+Qed.
+
+Lemma svfl_block_fields: forall from to v l g g',
+    graph_has_gen g to -> scan_vertex_for_loop from to v l g g' ->
+    forall x, graph_has_v g x -> block_fields (vlabel g x) = block_fields (vlabel g' x).
+Proof.
+  do 4 intro. revert from to v. induction l; intros; simpl; inversion H0; subst.
+  1: reflexivity. assert (graph_has_gen g2 to) by
+      (eapply fr_graph_has_gen in H4; [rewrite <- H4 |]; assumption).
+  assert (graph_has_v g2 x) by (eapply fr_graph_has_v in H4; eauto).
+  eapply (IHl from to _ g2) in H7; eauto. rewrite <- H7.
+  eapply fr_block_fields; eauto.
+Qed.
+
+Lemma svfl_block_mark: forall from to v l g g',
+    graph_has_gen g to -> scan_vertex_for_loop from to v l g g' ->
+    forall x, graph_has_v g x -> addr_gen x <> from ->
+              block_mark (vlabel g x) = block_mark (vlabel g' x).
+Proof.
+  do 4 intro. revert from to v. induction l; intros; simpl; inversion H0; subst.
+  1: reflexivity. assert (graph_has_gen g2 to) by
+      (eapply fr_graph_has_gen in H5; [rewrite <- H5 |]; assumption).
+  assert (graph_has_v g2 x) by (eapply fr_graph_has_v in H5; eauto).
+  eapply (IHl from to _ g2) in H8; eauto. rewrite <- H8.
+  eapply fr_block_mark; eauto.
+Qed.
+
+Lemma svfl_add_tail: forall from to v l roots i g1 g2 g3,
+    scan_vertex_for_loop from to v l g1 g2 ->
+    forward_relation from to 0
+                     (forward_p2forward_t (inr (v, Z.of_nat i)) roots g2) g2 g3 ->
+    scan_vertex_for_loop from to v (l +:: i) g1 g3.
+Proof.
+  do 4 intro. revert from to v. induction l; intros; inversion H; subst.
+  - simpl. rewrite forward_p2t_inr_roots in H0.
+    apply svfl_cons with g3. 1: assumption. constructor.
+  - simpl app. apply svfl_cons with g4. 1: assumption.
+    apply IHl with roots g2; assumption.
+Qed.
+
+Lemma svwl_add_tail_no_scan: forall from to l g1 g2 i,
+    scan_vertex_while_loop from to l g1 g2 -> gen_has_index g2 to i ->
+    no_scan g2 {| addr_gen := to; addr_block := i |} -> scan_vertex_while_loop from to (l +:: i) g1 g2.
+Proof.
+  do 3 intro. revert from to. induction l; intros; inversion H; subst.
+  - simpl. apply svwl_no_scan; assumption.
+  - simpl app. apply svwl_no_scan; try assumption. apply IHl; assumption.
+  - simpl app. apply svwl_scan with g3; try assumption. apply IHl; assumption.
+Qed.
+
+Lemma svwl_add_tail_scan: forall from to l g1 g2 g3 i,
+    scan_vertex_while_loop from to l g1 g2 -> gen_has_index g2 to i ->
+    ~ no_scan g2 {| addr_gen := to; addr_block := i |} ->
+    scan_vertex_for_loop
+      from to {| addr_gen := to; addr_block := i |}
+      (nat_inc_list (length (block_fields (vlabel g2 {| addr_gen := to; addr_block := i |}))))
+      g2 g3 ->
+    scan_vertex_while_loop from to (l +:: i) g1 g3.
+Proof.
+  do 3 intro. revert from to. induction l; intros; inversion H; subst.
+  - simpl. apply svwl_scan with g3; try assumption. constructor.
+  - simpl app. apply svwl_no_scan; try assumption. apply IHl with g2; assumption.
+  - simpl app. apply svwl_scan with g4; try assumption. apply IHl with g2; assumption.
+Qed.
+
+
+Definition do_generation_relation (from to: nat) (f_info: fun_info)
+           (roots roots': roots_t) (g g': HeapGraph): Prop := exists g1 g2,
+    forward_roots_relation from to f_info roots g roots' g1 /\
+    do_scan_relation from to (generation_block_count (nth_gen g to)) g1 g2 /\
+    g' = reset_graph from g2.
+
+
+Lemma svwl_graph_has_gen: forall from to l g1 g2,
+    graph_has_gen g1 to ->
+    scan_vertex_while_loop from to l g1 g2 ->
+    forall gen, graph_has_gen g1 gen <-> graph_has_gen g2 gen.
+Proof.
+  intros ? ? ?. induction l; intros; inversion H0; subst. 1: reflexivity.
+  - apply IHl; assumption.
+  - transitivity (graph_has_gen g3 gen).
+    + eapply svfl_graph_has_gen; eauto.
+    + apply IHl. 2: assumption. rewrite <- svfl_graph_has_gen; eauto.
+Qed.
+
+
+Lemma svfl_dst_unchanged: forall from to v l g1 g2,
+    graph_has_v g1 v -> block_mark (vlabel g1 v) = false -> addr_gen v <> from ->
+    (forall i,  In i l -> i < length (block_fields (vlabel g1 v)))%nat ->
+    graph_has_gen g1 to -> scan_vertex_for_loop from to v l g1 g2 ->
+    forall e, graph_has_v g1 (field_addr e) -> (forall i, In i l -> e <> {| field_addr := v; field_index := i |}) ->
+              dst g1 e = dst g2 e.
+Proof.
+  intros ? ? ? ?. induction l; intros; inversion H4; subst. 1: reflexivity.
+  transitivity (dst g3 e).
+  - eapply fr_O_dst_unchanged_field; eauto.
+    + simpl. intuition. rewrite Zlength_correct. apply inj_lt. apply H2.
+      left; reflexivity.
+    + apply H6. left; reflexivity.
+  - apply IHl; auto.
+    + eapply fr_graph_has_v; eauto.
+    + erewrite <- fr_block_mark; eauto.
+    + intros. erewrite <- fr_block_fields; eauto. apply H2. right; assumption.
+    + erewrite <- fr_graph_has_gen; eauto.
+    + eapply fr_graph_has_v; eauto.
+    + intros. apply H6. right; assumption.
+Qed.
+
+Lemma svwl_dst_unchanged: forall from to l g1 g2,
+    graph_has_gen g1 to -> scan_vertex_while_loop from to l g1 g2 ->
+    from <> to -> gen_unmarked g1 to ->
+    forall e, graph_has_v g1 (field_addr e) ->
+              (addr_gen (field_addr e) = to -> ~ In (addr_block (field_addr e)) l) ->
+              dst g1 e = dst g2 e.
+Proof.
+  intros. induction H0. 1: reflexivity.
+  - apply IHscan_vertex_while_loop; try assumption. intros. specialize (H4 H7).
+    intro. apply H4. right. assumption.
+  - transitivity (dst g2 e).
+    + eapply (svfl_dst_unchanged from to {| addr_gen := to; addr_block := i |}); eauto.
+      * split; assumption.
+      * intros. rewrite nat_inc_list_In_iff in H8. assumption.
+      * intros. destruct (Nat.eq_dec (addr_gen (field_addr e)) to).
+        -- specialize (H4 e0). intro. subst e. simpl in H4. apply H4. left; auto.
+        -- intro. subst e. simpl in n. apply n; reflexivity.
+    + apply IHscan_vertex_while_loop.
+      * erewrite <- svfl_graph_has_gen; eauto.
+      * eapply svfl_gen_unmarked; eauto.
+      * eapply svfl_graph_has_v; eauto.
+      * intros. specialize (H4 H8). intro. apply H4. right; assumption.
+Qed.
+
+Lemma svfl_gen_v_num_to: forall from to v l g1 g2,
+    graph_has_gen g1 to -> scan_vertex_for_loop from to v l g1 g2 ->
+    (gen_v_num g1 to <= gen_v_num g2 to)%nat.
+Proof.
+  intros ? ? ? ?. induction l; intros; inversion H0; subst. 1: lia.
+  assert (graph_has_gen g3 to) by (rewrite <- fr_graph_has_gen; eauto).
+  specialize (IHl _ _ H1 H6). transitivity (gen_v_num g3 to); auto.
+  eapply fr_O_gen_v_num_to; eauto.
+Qed.
+
+Lemma svfl_graph_has_v_inv: forall from to v l g1 g2,
+    graph_has_gen g1 to -> scan_vertex_for_loop from to v l g1 g2 ->
+    forall v2,
+      graph_has_v g2 v2 ->
+      graph_has_v g1 v2 \/
+      (addr_gen v2 = to /\ gen_v_num g1 to <= addr_block v2 < gen_v_num g2 to)%nat.
+Proof.
+  intros ? ? ? ?. induction l; intros; inversion H0; subst. 1: left; assumption.
+  assert (graph_has_gen g3 to) by (rewrite <- fr_graph_has_gen; eauto).
+  specialize (IHl _ _ H2 H7 _ H1). destruct IHl.
+  - eapply (fr_O_graph_has_v_inv from to _ g1 g3) in H4; eauto. destruct H4.
+    1: left; assumption. right. clear -H1 H4. unfold new_copied_v in H4. subst.
+    destruct H1. unfold gen_v_num. simpl in *. red in H0. lia.
+  - right. destruct H3. split. 1: assumption. destruct H5. split; auto.
+    eapply fr_O_gen_v_num_to in H4; [lia | assumption].
+Qed.
+
+Lemma svwl_graph_has_v: forall from to l g1 g2,
+    graph_has_gen g1 to -> scan_vertex_while_loop from to l g1 g2 ->
+    forall v, graph_has_v g1 v -> graph_has_v g2 v.
+Proof.
+  intros ? ? ?. induction l; intros; inversion H0; subst. 1: assumption.
+  1: eapply IHl; eauto. assert (graph_has_gen g3 to) by
+      (rewrite <- svfl_graph_has_gen; eauto). eapply IHl; eauto.
+  eapply (svfl_graph_has_v _ _ _ _ g1 g3); eauto.
+Qed.
+
+Lemma svwl_gen_v_num_to: forall from to l g1 g2,
+    graph_has_gen g1 to -> scan_vertex_while_loop from to l g1 g2 ->
+    (gen_v_num g1 to <= gen_v_num g2 to)%nat.
+Proof.
+  intros ? ? ?. induction l; intros; inversion H0; subst. 1: lia.
+  1: apply IHl; auto. transitivity (gen_v_num g3 to).
+  - eapply svfl_gen_v_num_to; eauto.
+  - apply IHl; auto. rewrite <- svfl_graph_has_gen; eauto.
+Qed.
+
+Lemma svwl_graph_has_v_inv: forall from to l g1 g2,
+    graph_has_gen g1 to -> scan_vertex_while_loop from to l g1 g2 ->
+    forall v,
+      graph_has_v g2 v ->
+      graph_has_v g1 v \/
+      (addr_gen v = to /\ gen_v_num g1 to <= addr_block v < gen_v_num g2 to)%nat.
+Proof.
+  intros ? ? ?. induction l; intros; inversion H0; subst. 1: left; assumption.
+  1: eapply IHl; eauto. assert (graph_has_gen g3 to) by
+      (rewrite <- svfl_graph_has_gen; eauto).
+  specialize (IHl _ _ H2 H9 _ H1). destruct IHl.
+  - eapply svfl_graph_has_v_inv in H6; eauto. destruct H6; [left|right]. 1: assumption.
+    destruct H6 as [? [? ?]]. split; [|split]; [assumption..|].
+    apply svwl_gen_v_num_to in H9; [lia | assumption].
+  - right. destruct H3 as [? [? ?]]. split; [|split]; try assumption.
+    apply svfl_gen_v_num_to in H6; [lia | assumption].
+Qed.
+
+Lemma svwl_block_fields: forall from to l g g',
+    graph_has_gen g to -> scan_vertex_while_loop from to l g g' ->
+    forall v, graph_has_v g v -> block_fields (vlabel g v) = block_fields (vlabel g' v).
+Proof.
+  do 3 intro. induction l; intros; inversion H0; subst. 1: reflexivity.
+  1: eapply IHl; eauto. erewrite <- (IHl g2 g'); eauto.
+  - eapply svfl_block_fields; eauto.
+  - rewrite <- svfl_graph_has_gen; eauto.
+  - eapply svfl_graph_has_v; eauto.
+Qed.
+
+Lemma svwl_gen2gen_no_edge: forall from to l g1 g2,
+    graph_has_gen g1 to -> from <> to -> gen_unmarked g1 to ->
+    scan_vertex_while_loop from to l g1 g2 ->
+    forall gen1 gen2, gen1 <> to -> gen2gen_no_edge g1 gen1 gen2 ->
+                      gen2gen_no_edge g2 gen1 gen2.
+Proof.
+  intros. unfold gen2gen_no_edge in *. intros. destruct H5. simpl in H5.
+  eapply svwl_graph_has_v_inv in H5; eauto. simpl in H5. destruct H5 as [? | [? ?]].
+  2: contradiction. erewrite <- svwl_dst_unchanged; eauto.
+  apply H4. split; simpl in *. 1: assumption.
+  cut (get_edges g1 {| addr_gen := gen1 ; addr_block := vidx |} = get_edges g2 {| addr_gen := gen1 ; addr_block := vidx |}).
+  + intros; rewrite H7; assumption.
+  + unfold get_edges. unfold make_fields. erewrite svwl_block_fields; eauto.
+Qed.
+
+
+Lemma svfl_dst_changed: forall from to v l g1 g2,
+    graph_has_v g1 v -> block_mark (vlabel g1 v) = false -> addr_gen v <> from ->
+    copy_compatible g1 -> no_dangling_dst g1 -> from <> to ->
+    (forall i,  In i l -> i < length (block_fields (vlabel g1 v)))%nat -> NoDup l ->
+    graph_has_gen g1 to -> scan_vertex_for_loop from to v l g1 g2 ->
+    forall e i, In i l -> Znth (Z.of_nat i) (make_fields g2 v) = inr e ->
+                addr_gen (dst g2 e) <> from.
+Proof.
+  intros ? ? ? ?. induction l; intros; inversion H8; subst. 1: inversion H9.
+  assert (e = {| field_addr := v ; field_index := i |}). {
+    apply make_fields_Znth_edge in H10. 1: rewrite Nat2Z.id in H10; assumption.
+    split. 1: lia. rewrite Zlength_correct. apply inj_lt.
+    erewrite <- svfl_block_fields; eauto. }
+  assert (graph_has_v g3 v) by (eapply fr_graph_has_v; eauto).
+  assert (block_mark (vlabel g3 v) = false) by (erewrite <- fr_block_mark; eauto).
+  assert (graph_has_gen g3 to) by (erewrite <- fr_graph_has_gen; eauto).
+  assert (forall j : nat, In j l -> j < Datatypes.length (block_fields (vlabel g3 v)))%nat. {
+    intros. erewrite <- (fr_block_fields _ _ _ _ g1); eauto. apply H5.
+    right; assumption. } simpl in H9. destruct H9.
+  - subst a. cut (addr_gen (dst g3 e) <> from).
+    + intros. cut (dst g2 e = dst g3 e). 1: intro HS; rewrite HS; assumption.
+      symmetry. apply (svfl_dst_unchanged from to v l); auto.
+      * subst e; simpl; assumption.
+      * intros. subst e. intro. inversion H11. subst. apply NoDup_cons_2 in H6.
+        contradiction.
+    + eapply (fr_O_dst_changed_field from to); eauto.
+      * simpl. intuition. rewrite Zlength_correct. apply inj_lt. apply H5.
+        left; reflexivity.
+      * unfold make_fields in H8 |-*. erewrite svfl_block_fields; eauto.
+  - eapply (IHl g3); eauto.
+    + eapply (fr_copy_compatible _ _ _ _ g1); eauto.
+    + eapply (fr_O_no_dangling_dst _ _ _ g1); eauto.
+      * simpl. intuition. rewrite Zlength_correct. apply inj_lt. apply H5.
+        left; reflexivity.
+      * simpl. constructor.
+    + apply NoDup_cons_1 in H6; assumption.
+Qed.
+
+Lemma svfl_no_edge2from: forall from to v g1 g2,
+    graph_has_v g1 v -> block_mark (vlabel g1 v) = false -> addr_gen v <> from ->
+    copy_compatible g1 -> no_dangling_dst g1 -> from <> to -> graph_has_gen g1 to ->
+    scan_vertex_for_loop
+      from to v (nat_inc_list (length (block_fields (vlabel g1 v)))) g1 g2 ->
+    forall e, In e (get_edges g2 v) -> addr_gen (dst g2 e) <> from.
+Proof.
+  intros. unfold get_edges in H7. rewrite <- filter_sum_right_In_iff in H7.
+  apply In_Znth in H7. destruct H7 as [i [? ?]].
+  rewrite <- (Z2Nat.id i) in H8 by lia. eapply svfl_dst_changed; eauto.
+  - intros. rewrite nat_inc_list_In_iff in H9. assumption.
+  - apply nat_inc_list_NoDup.
+  - rewrite nat_inc_list_In_iff. rewrite make_fields_eq_length in H7.
+    erewrite svfl_block_fields; eauto. rewrite <- ZtoNat_Zlength.
+    apply Z2Nat.inj_lt; lia.
+Qed.
